**Definition:** A Language $L\in DSPACE(s(n))$ if $\exists$ TM $M$ s.t. $L=L(M)$, and on every input $x$ of length $n$, $M$ halts and uses at most $O(s(n))$ cells on the tape. $(s(n) \geq n)$

**Claim:** Any $L\in DSPACE(s(n))$ is also in $DTIME(2^{O(s(n))})$
**Proof:** We will use the notion of configurations to show this fact:
A TM Configuration = $(q,z_{pre},z_{post})$
On an input of length $n$, 
$\#$ of possible configurations $=|Q|\times |\Gamma|^{s(n)}\times s(n)$
Where $Q$ is the set of states, $\Gamma$ is the tape alphabet, and where $s(n)$ is the length of $z_{pre}$ and $z_{post}$

The above can be simplified to 
$=O(1)\times 2^{O(1)\cdot s(n)}\times s(n)$
$=2^{O(s(n))}$
So, the TM $M$, given that it halts, must halt in $2^{O(s(n))}$ steps

$P:=\cup_{c\geq 1}DTIME(n^{c})$
$PSPACE:=\cup_{c\geq 1}DSPACE(n^{c})$
$EXPTIME:=\cup_{c \geq 1}DTIME(2^{n^{c}})$

$DTIME(n)$ is in $DSPACE(n)$ is in $DTIME(2^{O(n)})$

**Claim:** $NP \subseteq PSPACE$
**Proof:**
Suppose $L \in NP$
Then, $\exists V(.,.)$ such that for some $c_{1}>0, V(x,y)$ runs in time $(|x|+|y|)^{c_{1}}$ and 
(i) if $x \in L$, $\exists y, |y| \leq |x|^{c_{2}}$ s.t. $V(x,y)=1$
(ii) if $x \notin L, \forall y, |y| \leq |x|^{c_{2}}, V(x,y) = 0$
Then, construct a TM
$M(x)$ {
1. Iterate over all $y$ of length $\leq |x|^{c_{2}}$
2. Run $V(x,y)$
3. If $V(x,y)=1$, accept $x$,
4. Reject $x$;
}

**Time Complexity of $M$:**
$2^{O(|x|^{c_{2}})}\cdot (|x|+|x|^{c_{2}})^{c_{1}}$
$=2^{O(|x|^{c_{2}})}\cdot |x|^c_{1}c_{2}$
$=2^{O(|x|^{c_{2}})}$

Any language $L\in NP$ can be decided in time $2^{O(n^{c})}$ for some $c > 0$
$\implies NP \subseteq EXPTIME$
for any constants $\alpha, p>0$
$n^{B}=O(2^{n^{\alpha}})$
$n^{100}=O(2^{n^{0.001}})$

Total space used $=$ space for $y$ + space for executing $V(x,y)$ once
$=|x|^{c_{2}}+(|x|+|x|^{c_{2}})^{c_{1}}$
$=O(|x|^{c_{1}c_{2}})$

**Recurrence:**
$F(1)=1$; $F(2)=1$; $F(j)=F(j-1)+F(j-2)$
$Fib(j)${
If $j=1$ or $j=2$, return $1$;
Else, return $(F(j-1)+F(j-2))$
}

$\tau(j)=\tau(j-1)+\tau(j-2)$
$\tau \approx(\frac{\sqrt{5}+1}{2})^{j}$

$F(j)$ {
	Initialize $F(1)=F(i)=1$
	For ($l=3$ to $j$){
		$F(l)=F(l-1)+F(l-2)$;
	}
	return $F(j)$
}

